shift_rows/sub_bytes commutivity (#382)
* SubBytes - Vector.t -> list

In order to simplify the proof that sub_bytes and shift_rows commute,
it's better to have these two functions share the same representation.

Note that sub bytes is special in that the definition works whether the
data input is in row-major or column-major order. So, in the test here,
we interpret it to be a list of rows, and this makes its commutivity
with shift_rows definable without format conversions. Once we have mix
columns defined, that commutavity property might be defined without
format conversions as well, and we can prove 'transpose (sub_bytes x)
= sub_bytes (transpose x)'.

* Commutivity proof for shift_rows/sub_bytes.

In order to make this work, shift_rows has been generalized to
shift_rows_start, which can be thought of as the shift_rows
transformation of the end of a list of rows.

* aes/Spec - fixing missing license header header

Files missing starting (***...***) line, and it has spread like a virus.

silveroak-opentitan/aes/Spec/CommuteProperties.v
@@ -17,41 +17,56 @@
 Require Import Coq.Init.Byte.
 Require Import Coq.Lists.List.
 
+Require Import AesSpec.ShiftRows.
+Require Import AesSpec.SubBytes.
 Require Import AesSpec.Sbox.
-Require Import Cava.ListUtils.
 
 Section Spec.
-  Variables bytes_per_word Nb : nat.
-  Local Notation word := (list byte) (only parsing).
-  Local Notation state := (list word) (only parsing).
-
-  Definition sub_bytes : state -> state :=
-    map (map forward_sbox).
-
-  Definition inv_sub_bytes : state -> state :=
-    map (map inverse_sbox).
-
   Section Properties.
-
-    Lemma inverse_sbox_prop (x : byte) : inverse_sbox (forward_sbox x) = x.
+    Lemma sub_byte_shift_row_once_comm : forall row,
+      shift_row_once (map forward_sbox row) =
+      map forward_sbox (shift_row_once row).
     Proof.
-      destruct x; reflexivity.
-    Qed.
-
-    Theorem inverse_sub_bytes (x : state) :
-      inv_sub_bytes (sub_bytes x) = x.
-    Proof.
-      unfold inv_sub_bytes.
-      unfold sub_bytes.
-      induction x; [reflexivity|].
+      intros.
+      destruct row; [reflexivity|].
       simpl.
-      rewrite IHx.
-      rewrite map_map.
-      rewrite map_id_ext.
-      { reflexivity. }
-      { intro b.
-        destruct b; reflexivity. }
+      rewrite map_app.
+      reflexivity.
     Qed.
 
+    Lemma sub_byte_shift_row_comm : forall row shift,
+      shift_row (map forward_sbox row) shift =
+      map forward_sbox (shift_row row shift).
+    Proof.
+      intros.
+      generalize dependent row.
+      induction shift; [reflexivity|].
+      intros.
+      simpl.
+      rewrite <- IHshift.
+      rewrite sub_byte_shift_row_once_comm.
+      reflexivity.
+    Qed.
+
+    Lemma sub_bytes_shift_rows_start_comm : forall st n,
+      shift_rows_start (sub_bytes st) n =
+      sub_bytes (shift_rows_start st n).
+    Proof.
+      induction st; [reflexivity|].
+      intro n.
+      unfold shift_rows_start.
+      simpl.
+      rewrite sub_byte_shift_row_comm.
+      unfold shift_rows_start in IHst.
+      rewrite IHst.
+      reflexivity.
+    Qed.
+
+    Theorem sub_bytes_shift_rows_comm : forall st,
+      shift_rows (sub_bytes st) = sub_bytes (shift_rows st).
+    Proof.
+      intros.
+      apply (sub_bytes_shift_rows_start_comm st 0).
+    Qed.
   End Properties.
 End Spec.
